encoding derive and spec

theories/util.v
@@ -51,6 +51,42 @@ Proof.
   inversion Hi; subst; clear Hi. lia.
 Qed.
 
+(* TODO: merge index_range with nat_range *)
+Fixpoint index_range (n : nat) :=
+  match n with
+  | 0 => []
+  | S n' => index_range n' ++ [n']
+  end.
+
+Lemma index_range_length n :
+  length (index_range n) = n.
+Proof.
+  induction n => //=.
+  rewrite app_length /=. lia.
+Qed.
+
+Lemma index_range_lookup n i :
+  i < n →
+  index_range n !! i = Some i.
+Proof.
+  intros. induction n; first lia.
+  simpl. destruct (decide (i = n)) as [->|].
+  - rewrite lookup_app_r index_range_length //.
+    by rewrite Nat.sub_diag.
+  - have ? : i < n by lia.
+    rewrite lookup_app_l ?index_range_length; naive_solver.
+Qed.
+
+Lemma index_range_elem_of n x :
+  x ∈ index_range n → 0 ≤ x < n.
+Proof.
+  intros Hx. apply elem_of_list_lookup in Hx as [i Hi].
+  have ? : i < n.
+  { rewrite <- index_range_length. eapply lookup_lt_Some; eauto. }
+  rewrite index_range_lookup in Hi => //.
+  inversion Hi; subst; clear Hi. lia.
+Qed.
+
 Program Fixpoint big_or {A : Type} (l : list A) (P : {x : A & x ∈ l} → bool) : bool :=
     match l with
     | [] => false
