theories/encoding.v
@@ -1,0 +1,169 @@
+From stdpp Require Import relations.
+From Coq Require Import ssreflect.
+From ambig Require Import grammar decidability util ambiguity acyclic.
+
+Section encoding.
+
+  Variable Σ N : Type.
+  Context `{EqDecision Σ}.
+  Context `{EqDecision N}.
+
+  Variable G : grammar Σ N.
+  Context `{acyclic G}.
+
+  (* sat model *)
+
+  Record model := {
+    term : nat → Σ;
+    line : nat → nat;
+    col : nat → nat;
+    can_derive : N → nat (* start (inclusive) *) → nat (* length *) → bool;
+    can_reach_from : N → nat (* start (inclusive) *) → nat (* length *) → bool;
+  }.
+
+  Fixpoint decode m x δ : sentence Σ :=
+    match δ with
+    | 0 => []
+    | S n => term m x @ (line m x, col m x) :: decode m (S x) n
+    end.
+
+  Lemma decode_length m x δ :
+    length (decode m x δ) = δ.
+  Proof.
+    generalize dependent x.
+    induction δ => x //=.
+    naive_solver.
+  Qed.
+
+  Lemma decode_merge m x δ δ' :
+    decode m x δ ++ decode m (x + δ) δ' = decode m x (δ + δ').
+  Proof.
+    generalize dependent x.
+    induction δ as [|n IHn] => x /=.
+    - by rewrite -plus_n_O.
+    - rewrite <- IHn.
+      have -> : x + S n = S x + n by lia.
+      done.
+  Qed.
+
+  (* formula: a predicate over a model *)
+
+  Definition formula : Type := model → Prop.
+
+  (* encoding derivation *)
+
+  Definition Φ_derive k : formula := λ m,
+    ∀ A x δ, 0 < δ (* nonempty *) → x + δ ≤ k →
+      can_derive m A x δ = true ↔ Exists (λ α,
+        match α with
+        | ε => False (* not consider [] *)
+        | atom a => δ = 1 ∧ term m x = a
+        | unary B φ => apply₁ φ (decode m x δ) = true ∧ can_derive m B x δ = true
+        | binary Bl Br φ =>
+          (G ⊨ Bl ⇒ [] ∧ can_derive m Br x δ = true) ∨
+          (G ⊨ Br ⇒ [] ∧ can_derive m Bl x δ = true) ∨
+          (∃ δ', 0 < δ' < δ ∧
+            can_derive m Bl x δ' = true ∧
+            can_derive m Br (x + δ') (δ - δ') = true ∧
+            apply₂ φ (decode m x δ') (decode m (x + δ') (δ - δ')) = true)
+        end
+      ) (clauses G A).
+
+  Notation "⟨ x , y ⟩" := (existT x y).
+
+  Lemma list_nonempty_length {A} (l : list A) :
+    l ≠ [] ↔ 0 < length l.
+  Admitted.
+
+  Lemma Φ_derive_spec k m :
+    Φ_derive k m →
+    ∀ A x δ, 0 < δ → x + δ ≤ k →
+      can_derive m A x δ = true ↔ G ⊨ A ⇒ decode m x δ.
+  Proof.
+    intros HΦ A x δ ? ?. rewrite -check_derive_spec.
+    (* induction on range length *)
+    generalize dependent A.
+    generalize dependent x.
+    induction δ as [δ IHδ] using lt_wf_ind => x Hk A.
+    (* induction on nonterminal *)
+    have Hwf : wf (flip (succ G)) by apply acyclic_succ_flip_wf.
+    induction A as [A IHA] using (well_founded_induction Hwf).
+    (* rewrite definition *)
+    rewrite HΦ; [|done..].
+    rewrite check_derive_equation big_or_true Exists_exists.
+    split.
+    - (* -> *)
+      intros [α [Hp Hα]]. exists ⟨α, Hp⟩.
+      case_match => //.
+      3: destruct Hα as [Hα|[Hα|Hα]].
+      + destruct Hα as [-> ?]. repeat case_match => //.
+        apply bool_decide_eq_true. naive_solver.
+      + destruct Hα as [? ?].
+        apply andb_true_iff. split => //.
+        clear IHδ. apply IHA => //. eapply succ_unary; eauto.
+      + destruct Hα as [Hn ?].
+        apply orb_true_iff; left. apply orb_true_iff; left.
+        apply when_true. exists Hn.
+        clear IHδ. apply IHA => //. eapply succ_right; eauto.
+      + destruct Hα as [Hn ?].
+        apply orb_true_iff; left. apply orb_true_iff; right.
+        apply when_true. exists Hn.
+        clear IHδ. apply IHA => //. eapply succ_left; eauto.
+      + destruct Hα as [δ' [? [? [? ?]]]].
+        apply orb_true_iff; right.
+        apply big_or_true.
+        have Hpar : (decode m x δ', decode m (x + δ') (δ - δ')) ∈ nonempty_partition (decode m x δ).
+        { eapply nonempty_partition_spec; eauto.
+          split. rewrite decode_merge. f_equal. lia.
+          split. all: apply list_nonempty_length.
+          all: rewrite decode_length; lia. }
+        exists ⟨(decode m x δ', decode m (x + δ') (δ - δ')), Hpar⟩.
+        apply andb_true_iff. split.
+        apply andb_true_iff. split => //.
+        all: clear IHA; apply IHδ; [lia..|done].
+      - (* <- *)
+        intros [[α Hp] Hα]. exists α. split; first by apply Hp.
+        case_match.
+        4: apply orb_true_iff in Hα as [Hα|Hα]; first apply orb_true_iff in Hα as [Hα|Hα].
+        + apply bool_decide_eq_true in Hα.
+          have ? : decode m x δ ≠ [].
+          { apply list_nonempty_length. rewrite decode_length. lia. }
+          contradiction.
+        + repeat case_match => //.
+          apply bool_decide_eq_true in Hα.
+          have ? : δ = 1.
+          { have Hl : length (decode m x δ) = 1 by rewrite Heqs.
+            by rewrite decode_length in Hl. }
+          subst. split => //. naive_solver.
+        + apply andb_true_iff in Hα as [? ?]. split => //.
+          clear IHδ. apply IHA => //. eapply succ_unary; eauto.
+        + apply when_true in Hα as [? ?]. left. split => //.
+          clear IHδ. apply IHA => //. eapply succ_right; eauto.
+        + apply when_true in Hα as [? ?]. right. left. split => //.
+          clear IHδ. apply IHA => //. eapply succ_left; eauto.
+        + apply big_or_true in Hα as [[[wl wr] Hw] Hα].
+          apply andb_true_iff in Hα as [Hα ?].
+          apply andb_true_iff in Hα as [? ?].
+          right. right.
+          eapply nonempty_partition_spec in Hw as [Hw [? ?]]; eauto.
+          exists (length wl).
+          have ? : length (decode m x δ) = δ by rewrite decode_length.
+          have ? : length (decode m x δ) = length wl + length wr
+            by rewrite Hw app_length.
+          have ? : 0 < length wl by apply list_nonempty_length.
+          have ? : 0 < length wr by apply list_nonempty_length.
+          have Hw' : decode m x δ = decode m x (length wl) ++
+            decode m (x + length wl) (δ - length wl).
+            by rewrite decode_merge; f_equal; lia.
+          have [Hwl Hwr] : decode m x (length wl) = wl ∧
+                           decode m (x + length wl) (δ - length wl) = wr.
+          { rewrite Hw in Hw'. apply app_inj_1 => //. by rewrite decode_length.  }
+          rewrite Hwl Hwr.
+          split; first lia. repeat split => //.
+          1,2: clear IHA; apply IHδ; [lia..|].
+          by rewrite Hwl. by rewrite Hwr.
+    (* TODO: why this is shelved? *)
+    Unshelve. done.
+  Qed.
+
+End encoding.
